\begin{tikzpicture}[scale=1]
		
	\node (fcp) at (0,0) {$F(c')$};
	\node (gcp) at (4,0) {$G(c')$};
	\node (fc) at (0,3) {$F(c)$};
	\node (gc) at (4,3) {$G(c)$};
	
	\path[->,font=\scriptsize]
		(fc) edge node[above]{$[(F(c);\sigma_c;G(c))]$} (gc)
		(fcp) edge node[below]{$[(F(c');\sigma_{c'};G(c'))]$} (gcp)
		(fcp) edge node[left]{$[(F(c);F(f);F(c'))]^{-1} = \Lambda(F)([(c';\bar{f};c)])$} (fc)
		(gcp) edge node[right]{$\Lambda(G)([(c';\bar{f};c)]) = [(G(c);G(f);G(c'))]^{-1}$} (gc);
			
\end{tikzpicture}